Parametrize FlatImp.exec by compiler phase
The spilling phase adds some boilerplate inside functions and around
function calls, so we need to account for it by making things
artificially more expensive before the spilling phase.

In an effort to avoid monolithic commits, this is a partial commit, so
the code definitely doesn't compile in the current state since lots of
things changed as a side effect.

There are a few comments that say "cost_something constraint:", which
document the various constraints on the magic numbers chosen as upper
bounds for the costs (100, 95, 50). These should probably change to
better numbers at some point.

compiler/src/compiler/FlatImp.v
@@ -26,6 +26,10 @@ Inductive bbinop: Type :=
 | BLtu
 | BGeu.
 
+Inductive compphase: Type :=
+| PreSpill
+| PostSpill.
+
 Section Syntax.
   Context {varname: Type}.
 
@@ -282,6 +286,7 @@ Module exec.
             {env_ok: map.ok env}
             {ext_spec_ok: ext_spec.ok ext_spec}.
 
+    Variable (phase: compphase).
     Variable (isReg: varname -> bool).
 
     Variable (e: env).
@@ -298,6 +303,26 @@ Module exec.
       end.
 
     (* Helper functions for computing costs of instructions *)
+    Definition cost_SInteract mc :=
+      match phase with
+      | PreSpill => (addMetricInstructions 100 (addMetricJumps 100 (addMetricStores 100 (addMetricLoads 100 mc))))
+      | PostSpill => (addMetricInstructions 50 (addMetricJumps 50 (addMetricStores 50 (addMetricLoads 50 mc))))
+      end.
+
+    Definition cost_SCall_internal mc :=
+      match phase with
+      | PreSpill => addMetricInstructions 100 (addMetricJumps 100 (addMetricLoads 100 (addMetricStores 100 mc)))
+      | PostSpill => addMetricInstructions 50 (addMetricJumps 50 (addMetricLoads 50 (addMetricStores 50 mc)))
+      end.
+
+    Definition cost_SCall_external mc :=
+      match phase with
+      | PreSpill => addMetricInstructions 100 (addMetricJumps 100 (addMetricLoads 100 (addMetricStores 100 mc)))
+      | PostSpill => addMetricInstructions 50 (addMetricJumps 50 (addMetricLoads 50 (addMetricStores 50 mc)))
+      end.
+
+    (* TODO think about a non-fixed bound on the cost of function preamble and postamble *)
+
     Definition cost_SLoad x a mc :=
       match (isReg x, isReg a) with
       | (false, false) => (addMetricInstructions 3 (addMetricLoads 5 (addMetricStores 1 mc)))
@@ -412,24 +437,20 @@ Module exec.
             exists l', map.putmany_of_list_zip resvars resvals l = Some l' /\
             forall m', map.split m' mKeep mReceive ->
             post (((mGive, action, argvals), (mReceive, resvals)) :: t) m' l'
-                 (addMetricInstructions 100
-                 (addMetricJumps 100
-                 (addMetricStores 100
-                 (addMetricLoads 100 mc))))) ->
+                 (cost_SInteract mc)) ->
         exec (SInteract resvars action argvars) t m l mc post
     | call: forall t m l mc binds fname args params rets fbody argvs st0 post outcome,
         map.get e fname = Some (params, rets, fbody) ->
         map.getmany_of_list l args = Some argvs ->
         map.putmany_of_list_zip params argvs map.empty = Some st0 ->
-        exec fbody t m st0 (addMetricInstructions 100 (addMetricJumps 100 (addMetricLoads 100 (addMetricStores 100 mc)))) outcome ->
+        exec fbody t m st0 (cost_SCall_internal mc) outcome ->
         (forall t' m' mc' st1,
             outcome t' m' st1 mc' ->
             exists retvs l',
               map.getmany_of_list st1 rets = Some retvs /\
               map.putmany_of_list_zip binds retvs l = Some l' /\
-              post t' m' l' (addMetricInstructions 100 (addMetricJumps 100 (addMetricLoads 100 (addMetricStores 100 mc'))))) ->
+              post t' m' l' (cost_SCall_external mc')) ->
         exec (SCall binds fname args) t m l mc post
-        (* TODO think about a non-fixed bound on the cost of function preamble and postamble *)
     | load: forall t m l mc sz x a o v addr post,
         map.get l a = Some addr ->
         load sz m (word.add addr (word.of_Z o)) = Some v ->
@@ -531,12 +552,12 @@ Module exec.
         map.get e fname = Some (params, rets, fbody) ->
         map.getmany_of_list l args = Some argvs ->
         map.putmany_of_list_zip params argvs map.empty = Some st ->
-        exec fbody t m st (addMetricInstructions 100 (addMetricJumps 100 (addMetricLoads 100 (addMetricStores 100 mc))))
+        exec fbody t m st (cost_SCall_internal mc)
              (fun t' m' st' mc' =>
                 exists retvs l',
                   map.getmany_of_list st' rets = Some retvs /\
                     map.putmany_of_list_zip binds retvs l = Some l' /\
-                    post t' m' l' (addMetricInstructions 100 (addMetricJumps 100 (addMetricLoads 100 (addMetricStores 100 mc'))))) ->
+                    post t' m' l' (cost_SCall_external mc')) ->
       exec (SCall binds fname args) t m l mc post.
     Proof.
       intros. eapply call; try eassumption.
@@ -702,16 +723,17 @@ Section FlatImp2.
           {env_ok: map.ok env}
           {ext_spec_ok: ext_spec.ok ext_spec}.
 
+  Variable (phase: compphase).
   Variable (isReg: varname -> bool).
   
   Definition SimState: Type := trace * mem * locals * MetricLog.
   Definition SimExec(e: env)(c: stmt varname): SimState -> (SimState -> Prop) -> Prop :=
     fun '(t, m, l, mc) post =>
-      exec isReg e c t m l mc (fun t' m' l' mc' => post (t', m', l', mc')).
+      exec phase isReg e c t m l mc (fun t' m' l' mc' => post (t', m', l', mc')).
 
   Lemma modVarsSound: forall e s initialT (initialSt: locals) initialM (initialMc: MetricLog) post,
-      exec isReg e s initialT initialM initialSt initialMc post ->
-      exec isReg e s initialT initialM initialSt initialMc
+      exec phase isReg e s initialT initialM initialSt initialMc post ->
+      exec phase isReg e s initialT initialM initialSt initialMc
            (fun finalT finalM finalSt _ => map.only_differ initialSt (modVars s) finalSt).
   Proof.
     induction 1;
@@ -775,6 +797,3 @@ Definition isRegZ (var : Z) : bool :=
 
 Definition isRegStr (var : String.string) : bool :=
   String.prefix "reg_" var.
-
-
-
