compiler/src/compiler/FlatToRiscvCommon.v
@@ -288,7 +288,7 @@ Section WithParameters.
       exists pos, map.get finfo f = Some pos /\ pos mod 4 = 0.
 
   Local Notation stmt := (stmt Z).
-  Local Notation exec := (exec isRegZ). 
+  Local Notation exec := (exec PostSpill isRegZ). 
   
   (* note: [e_impl_reduced] and [funnames] will shrink one function at a time each time
      we enter a new function body, to make sure functions cannot call themselves, while
